src/unitb/models/simple.lean
@@ -5,6 +5,8 @@ import unitb.logic
 
 import util.logic
 
+local notation `♯` x := cast (by simp) x
+
 namespace simple
 
 open unitb
@@ -28,7 +30,7 @@ s.first ⊨ p
 def is_step (s : program) (σ σ' : α) : Prop := σ' = s.step σ
 
 def program.transient (s : program) (p q : pred) : Prop :=
-⊩ ⟦is_step s⟧ ⟶ •p ⟶ •q ⟶ ⊙-•q
+∀ v, ⊩ ⟦v | is_step s⟧ ⟶ p!v ⟶ q!v ⟶ ⊙-(q!v)
 
 def program.unless (s : program) (p q : pred) : Prop :=
 ∀ σ, σ ⊨ p ∧ ¬σ ⊨ p → s.step σ ⊨ p ∨ s.step σ ⊨ q
@@ -38,14 +40,18 @@ open temporal
 lemma program.transient_impl (s : program) {p q : pred}
   (H : p ⟹ -q)
 : s.transient p q :=
+begin intro,
 begin [temporal]
   intros STEP hp hq,
   exfalso,
   revert hq hp,
-  simp, rw [not_init],
+  simp,
   clear STEP,
   show _,
-  { revert Γ, change _ ⟹ _, monotonicity H, },
+  { revert Γ, change _ ⟹ _,
+    simp only [p_not_comp],
+    monotonicity H, },
+end
 end
 
 lemma program.transient_antimono (s : program) (p q p' q' : pred)
@@ -53,15 +59,14 @@ lemma program.transient_antimono (s : program) (p q p' q' : pred)
   (hq : q' ⟹ q)
   (T₀ : s.transient p q)
 : s.transient p' q' :=
+begin intro,
 begin [temporal]
-  replace hp := init_entails_init hp,
-  replace hq := init_entails_init hq,
   intros STEP hp' hq',
-  replace T₀ := T₀ Γ STEP (hp Γ hp') (hq Γ hq'),
-  revert T₀,
-  persistent,
-  monotonicity,
-  apply hq,
+  replace T₀ := T₀ v Γ STEP _ _,
+  apply_mono hq T₀,
+  apply_mono hp hp',
+  apply_mono hq hq',
+end
 end
 
 instance prog_is_system : system program :=
@@ -100,7 +105,7 @@ lemma leads_to_step
 : p ↦ q in program.mk init step :=
 begin
   apply leads_to.basis,
-  { lifted_pred [is_step,temporal.init,not_not_iff_self],
+  { intro, lifted_pred [is_step,not_not_iff_self],
     intros, specialize h _ a_1 a_2,
     simp [a,h], },
   { apply unless_step,
@@ -112,67 +117,64 @@ open nat
 
 open temporal
 
-def ex (s : program) : cpred α :=
-•eq s.first ⋀ ◻ ⟦ is_step s ⟧
+variables (s : program) (v : tvar α)
 
-lemma ex.safety (s : program)
-: ex s ⟹ ◻ ⟦ is_step s ⟧ :=
+def ex : cpred :=
+v ≃ s.first ⋀ ◻ ⟦ v | is_step s ⟧
+
+lemma ex.safety
+: ex s v ⟹ ◻ ⟦ v | is_step s ⟧ :=
 begin [temporal]
   intros h, apply h.right
 end
 
-def ex.witness (s : program) : stream α
-  | 0 := s.first
-  | (succ i) := s.step (ex.witness i)
+-- def ex.witness : tvar α :=
+-- tvar.mk s.first s.step
 
-lemma ex.witness_correct (s : program)
-: ex.witness s ⊨ ex s :=
+lemma ex.witness_correct
+: ⊩ ∃∃ w, ex s w :=
 begin
-  unfold ex, simp,
-  split,
-  { intro i,
-    simp [action,is_step,stream.drop],
-    refl },
-  { simp [temporal.init],
-    exact rfl }
+  have _inst : inhabited α := ⟨ s.first ⟩,
+  have := @witness_construction _ (whole ≃ ↑s.first) True (is_step s) _ _ _ _ _
+  ; try { revert this }
+  ; simp [is_step,ex],
 end
 
 section semantics
 
-variable {s : program}
-variable Γ : cpred α
+variable {s}
+variable Γ : cpred
 variables {p q : pred}
-variables H : Γ ⊢ ex s
+variable σ : tvar α
+variables H : Γ ⊢ ex s σ
 open temporal
 include H
 
 lemma init_sem
   (I₀ : init s p)
-: Γ ⊢ •p :=
+: Γ ⊢ p ! σ :=
 begin [temporal]
-  have H' := H.left,
-  revert H',
+  dsimp [init,system.init] at I₀,
+  replace H := H.left,
+  rw H,
   lifted_pred,
   show _ ,
-  { intros,
-    simp [temporal.init] at a ⊢,
-    rw ← a,
-    assumption },
+  { exact I₀, },
 end
 
 lemma transient.semantics
   (T₀ : transient' s p q)
-: Γ ⊢ ◻◇•p ⟶ ◻◇-•q :=
+: Γ ⊢ ◻◇(p!σ) ⟶ ◻◇-(q!σ) :=
 begin [temporal]
   intros Hp,
-  replace H := coincidence' (ex.safety s Γ H) Hp,
+  replace H := coincidence' (ex.safety s σ Γ H) Hp,
   rw ← eventually_eventually,
   revert H,
   monotonicity,
   { rw p_and_p_imp,
     intros Hs Hp,
-    cases predicate.em (•q) with Hq Hnq,
-    { apply T₀ Γ Hs Hp Hnq, },
+    cases predicate.em (q!σ) with Hq Hnq,
+    { apply T₀ σ Γ Hs Hp Hnq, },
     { apply Hq } },
 end
 
@@ -182,7 +184,7 @@ instance : system_sem program :=
   { (_ : system program) with
     ex := ex
   , safety := @ex.safety
-  , inhabited := λ p, ⟨ex.witness p, ex.witness_correct p⟩
+  , inhabited := ex.witness_correct
   , init_sem := @init_sem
   , transient_sem := @transient.semantics }
 
