src/unitb/refinement/basic.lean
@@ -17,15 +17,15 @@ variables {α β : Type u}
 variables {σ : Type u'}
 
 def refined (s s' : α) [system_sem α] : Prop :=
-system_sem.ex s' ⟹ system_sem.ex s
+∀ σ, system_sem.ex s' σ ⟹ system_sem.ex s σ
 
 infix ` ⊑ `:80 := refined
 
 def data_ref [system_sem α] [system_sem β]
-    (s : α)  (f : unitb.state α  → σ)
-    (s' : β) (g : unitb.state β  → σ) : Prop :=
-∀ τ : stream (unitb.state β),
-        τ  ⊨ system_sem.ex s'
-→ ∃ τ', τ' ⊨ system_sem.ex s ∧ (g ∘ τ) = (f ∘ τ')
+    (s : α)  (f : var (unitb.state α) σ)
+    (s' : β) (g : var (unitb.state β) σ) : Prop :=
+∀ σ' Γ,
+     Γ ⊢ system_sem.ex s' σ' →
+     Γ ⊢ ∃∃ σ, system_sem.ex s σ ⋀ (g ! σ') ≃ (f ! σ)
 
 end unitb.refinement
